x64: ArchVSpaceLookup_AI: prove vs_lookup_pages1_wellformed_order
Show that there is a measure on vs_refs, on which vs_lookup_pages1 is
strictly monotonically increasing.

We also prove various lemmas relating vs_lookup and vs_lookup_pages, and
valid_arch_objs.

There are many things previously proved in ArchRetype_AI and
ArchDetype_AI that are now broken because Xin's work overwrote some
things I also proved in ArchVSpace_AI. I'm not fixing them here.

proof/invariant-abstract/InvariantsPre_AI.thy
@@ -75,8 +75,8 @@ lemma obj_at_pspaceI:
   "\<lbrakk> obj_at P ref s; kheap s = kheap s' \<rbrakk> \<Longrightarrow> obj_at P ref s'"
   by (simp add: obj_at_def)
 
-abbreviation
-  "ko_at k \<equiv> obj_at (op = k)"
+abbreviation "ko_at k \<equiv> obj_at (op = k)"
+abbreviation "ako_at ako == ko_at (ArchObj ako)"
 
 lemma obj_atE:
   "\<lbrakk> obj_at P p s; \<And>ko. \<lbrakk> kheap s p = Some ko; P ko \<rbrakk> \<Longrightarrow> R \<rbrakk> \<Longrightarrow> R"
